git-svn-id: https://projects.brucker.ch/hol-testgen/svn/HOL-TestGen/trunk/hol-testgen@9780 3260e6d1-4efc-4170-b0a7-36055960796d

examples/Employee_DesignModel_UMLPart.thy
@@ -251,7 +251,6 @@ defs (overloaded) oclastype\<^isub>p\<^isub>e\<^isub>r\<^isub>s\<^isub>o\<^isub>
 defs (overloaded) oclastype\<^isub>p\<^isub>e\<^isub>r\<^isub>s\<^isub>o\<^isub>n_Person: 
         "(X::Person) .oclAsType(Person) \<equiv> X "  (* to avoid identity for null ? *)
 
-definition "oclastype\<^isub>p\<^isub>e\<^isub>r\<^isub>s\<^isub>o\<^isub>n_\<AA> u = (case u of in\<^isub>p\<^isub>e\<^isub>r\<^isub>s\<^isub>o\<^isub>n p \<Rightarrow> p | in\<^isub>o\<^isub>c\<^isub>l\<^isub>a\<^isub>n\<^isub>y (mk\<^isub>o\<^isub>c\<^isub>l\<^isub>a\<^isub>n\<^isub>y oid \<lfloor>(a,b)\<rfloor>) \<Rightarrow> mk\<^isub>p\<^isub>e\<^isub>r\<^isub>s\<^isub>o\<^isub>n oid a b)"
 
 lemmas [simp] =
  oclastype\<^isub>o\<^isub>c\<^isub>l\<^isub>a\<^isub>n\<^isub>y_OclAny
@@ -458,14 +457,15 @@ consts ocliskinfof\<^isub>p\<^isub>e\<^isub>r\<^isub>s\<^isub>o\<^isub>n :: "'\<
 defs (overloaded) ocliskindof\<^isub>o\<^isub>c\<^isub>l\<^isub>a\<^isub>n\<^isub>y_OclAny: 
         "(X::OclAny) .oclIsKindOf(OclAny) \<equiv> 
                    (\<lambda>\<tau>. case X \<tau> of 
-                              \<bottom>   \<Rightarrow> invalid \<tau>
+                              \<bottom> \<Rightarrow> invalid \<tau>
                             | _ \<Rightarrow> true \<tau>)" 
 
 defs (overloaded) ocliskindof\<^isub>o\<^isub>c\<^isub>l\<^isub>a\<^isub>n\<^isub>y_Person: 
         "(X::Person) .oclIsKindOf(OclAny) \<equiv> 
                    (\<lambda>\<tau>. case X \<tau> of 
-                              \<bottom>   \<Rightarrow> invalid \<tau>
-                            | _ \<Rightarrow> true \<tau>)"  (* for (* \<lfloor>\<lfloor>mk\<^isub>p\<^isub>e\<^isub>r\<^isub>s\<^isub>o\<^isub>n e oid _ \<rfloor>\<rfloor> \<Rightarrow> true \<tau> *) :  must have actual type Person otherwise  *)
+                              \<bottom> \<Rightarrow> invalid \<tau>
+                            | _\<Rightarrow> true \<tau>)"  
+(* for (* \<lfloor>\<lfloor>mk\<^isub>p\<^isub>e\<^isub>r\<^isub>s\<^isub>o\<^isub>n e oid _ \<rfloor>\<rfloor> \<Rightarrow> true \<tau> *) :  must have actual type Person otherwise  *)
 (* Unchecked; or better directly on the OCL - level ??? *)
 
 (* stricness, null-ness, cp, reduction-rules. *)
@@ -476,57 +476,70 @@ text{* Should be generated entirely from a class-diagram. *}
 
 typ "Person \<Rightarrow> Person"
 
-definition "get_oid fst_snd f oid = (\<lambda>\<tau>. case (heap (fst_snd \<tau>)) oid of
-                       \<lfloor> univ \<rfloor> \<Rightarrow> f (oclastype\<^isub>p\<^isub>e\<^isub>r\<^isub>s\<^isub>o\<^isub>n_\<AA> univ) \<tau>
-                     | _ \<Rightarrow> invalid \<tau>)"
+definition "eval_extract X f = (\<lambda> \<tau>. case X \<tau> of
+                                    \<bottom> \<Rightarrow> invalid \<tau>   (* exception propagation *)
+                               | \<lfloor>  \<bottom> \<rfloor> \<Rightarrow> invalid \<tau> (* dereferencing null pointer *)
+                               | \<lfloor>\<lfloor> obj \<rfloor>\<rfloor> \<Rightarrow> f (oid_of obj) \<tau>)"
 
-definition "access X f = (\<lambda> \<tau>. case X \<tau> of
-               \<bottom> \<Rightarrow> invalid \<tau> (* exception propagation *)
-          | \<lfloor>  \<bottom> \<rfloor> \<Rightarrow> invalid \<tau> (* dereferencing null pointer *)
-          | \<lfloor>\<lfloor> obj \<rfloor>\<rfloor> \<Rightarrow> f (oid_of obj) \<tau>)"
+
+definition "deref\<^isub>o\<^isub>i\<^isub>d fst_snd f oid = (\<lambda>\<tau>. case (heap (fst_snd \<tau>)) oid of
+                       \<lfloor> in\<^isub>p\<^isub>e\<^isub>r\<^isub>s\<^isub>o\<^isub>n obj \<rfloor> \<Rightarrow> f ( obj) \<tau>
+                     | _       \<Rightarrow> invalid \<tau>)"
+text{* pointer undefined in state or not referencing a type conform object representation *}
 
 (*
-definition "access2 X f =
-               (\<lambda>(\<sigma>,\<sigma>'). (let Ob = (I\<lbrakk>X\<rbrakk>(\<sigma>,\<sigma>')) in
-                            if (Ob=\<bottom>) \<or> (Ob=\<lfloor>\<bottom>\<rfloor>) \<or> (oid_of \<lceil>\<lceil>Ob\<rceil>\<rceil>) \<in> (dom \<sigma>') then invalid(\<sigma>,\<sigma>')
-                            else undefined))"
+definition "oclastype\<^isub>p\<^isub>e\<^isub>r\<^isub>s\<^isub>o\<^isub>n_\<AA> u = (case u of in\<^isub>p\<^isub>e\<^isub>r\<^isub>s\<^isub>o\<^isub>n p \<Rightarrow>  p 
+                                          | in\<^isub>o\<^isub>c\<^isub>l\<^isub>a\<^isub>n\<^isub>y (mk\<^isub>o\<^isub>c\<^isub>l\<^isub>a\<^isub>n\<^isub>y oid \<lfloor>(a,b)\<rfloor>) \<Rightarrow> (mk\<^isub>p\<^isub>e\<^isub>r\<^isub>s\<^isub>o\<^isub>n oid a b))"
 *)
 
-definition "access_to_boss f = (\<lambda> X. case X of 
-                     mk\<^isub>p\<^isub>e\<^isub>r\<^isub>s\<^isub>o\<^isub>n _ _ \<bottom> \<Rightarrow> null (* object contains null pointer *)
-                   | mk\<^isub>p\<^isub>e\<^isub>r\<^isub>s\<^isub>o\<^isub>n _ _ \<lfloor>boss\<rfloor> \<Rightarrow> f (\<lambda>x _. \<lfloor>\<lfloor>x\<rfloor>\<rfloor>) boss)"
+definition "select\<^isub>b\<^isub>o\<^isub>s\<^isub>s f = (\<lambda> X. case X of 
+                     (mk\<^isub>p\<^isub>e\<^isub>r\<^isub>s\<^isub>o\<^isub>n _ _ \<bottom>) \<Rightarrow> null  (* object contains null pointer *)
+                   | (mk\<^isub>p\<^isub>e\<^isub>r\<^isub>s\<^isub>o\<^isub>n _ _ \<lfloor>boss\<rfloor>) \<Rightarrow> f (\<lambda>x _. \<lfloor>\<lfloor>x\<rfloor>\<rfloor>) boss)"
 
-definition "access_to_salary = (\<lambda> X _. case X of mk\<^isub>p\<^isub>e\<^isub>r\<^isub>s\<^isub>o\<^isub>n _ i _ \<Rightarrow> \<lfloor>i\<rfloor>)"
 
-definition "at_pre = get_oid fst"
-definition "at_post = get_oid snd"
+definition "select\<^isub>s\<^isub>a\<^isub>l\<^isub>a\<^isub>r\<^isub>y f = (\<lambda> X. case X of
+                     (mk\<^isub>p\<^isub>e\<^isub>r\<^isub>s\<^isub>o\<^isub>n _ i _) \<Rightarrow> f (\<lambda>x _. \<lfloor>x\<rfloor>) i)"
 
-lemmas [simp] =
- access_def
- access_to_boss_def
- access_to_salary_def
+
+definition "in_pre_state = fst"
+definition "in_post_state = snd"
+
+definition "reconst_basetype = (\<lambda> convert x. convert x)"
 
 fun dot_boss:: "Person \<Rightarrow> Person"  ("(1(_).boss)" 50)
-  where "(X).boss = access X (at_post (access_to_boss at_post))"
+  where "(X).boss = eval_extract X 
+                      (deref\<^isub>o\<^isub>i\<^isub>d in_post_state 
+                         (select\<^isub>b\<^isub>o\<^isub>s\<^isub>s 
+                            (deref\<^isub>o\<^isub>i\<^isub>d in_post_state)))"
 
 fun dot_salary:: "Person \<Rightarrow> Integer"  ("(1(_).salary)" 50)
-  where "(X).salary = access X (at_post access_to_salary)"
+  where "(X).salary = eval_extract X 
+                       (deref\<^isub>o\<^isub>i\<^isub>d in_post_state 
+                          (select\<^isub>s\<^isub>a\<^isub>l\<^isub>a\<^isub>r\<^isub>y 
+                             reconst_basetype))"
 
 fun dot_boss_at_pre:: "Person \<Rightarrow> Person"  ("(1(_).boss@pre)" 50)
-  where "(X).boss@pre = access X (at_pre (access_to_boss at_pre))"
+  where "(X).boss@pre = eval_extract X 
+                         (deref\<^isub>o\<^isub>i\<^isub>d in_pre_state 
+                            (select\<^isub>b\<^isub>o\<^isub>s\<^isub>s 
+                               (deref\<^isub>o\<^isub>i\<^isub>d in_pre_state)))"
   (* | \<lfloor>\<lfloor> mk\<^isub>p\<^isub>e\<^isub>r\<^isub>s\<^isub>o\<^isub>n _ _ \<bottom> \<rfloor>\<rfloor> \<Rightarrow> null (* object contains null pointer. REALLY ? 
-                                          And if this pointer was defined in the pre-state ?*) *)
+                                     And if this pointer was defined in the pre-state ?*) *)
 
 fun dot_salary_at_pre:: "Person \<Rightarrow> Integer"  ("(1(_).salary@pre)" 50)
-  where "(X).salary@pre = access X (at_pre access_to_salary)"
+  where "(X).salary@pre = eval_extract X 
+                            (deref\<^isub>o\<^isub>i\<^isub>d in_pre_state 
+                               (select\<^isub>s\<^isub>a\<^isub>l\<^isub>a\<^isub>r\<^isub>y 
+                                   reconst_basetype))"
 
-lemma cp_dot_boss: "((X).boss) \<tau> = ((\<lambda>_. X \<tau>).boss) \<tau>" by(simp)
 
-lemma cp_dot_salary: "((X).salary) \<tau> = ((\<lambda>_. X \<tau>).salary) \<tau>" by(simp)
+lemma cp_dot_boss: "((X).boss) \<tau> = ((\<lambda>_. X \<tau>).boss) \<tau>" by(simp add: eval_extract_def)
 
-lemma cp_dot_boss_at_pre: "((X).boss@pre) \<tau> = ((\<lambda>_. X \<tau>).boss@pre) \<tau>" by(simp)
+lemma cp_dot_salary: "((X).salary) \<tau> = ((\<lambda>_. X \<tau>).salary) \<tau>" by(simp add: eval_extract_def)
 
-lemma cp_dot_boss_pre: "((X).salary@pre) \<tau> = ((\<lambda>_. X \<tau>).salary@pre) \<tau>" by(simp)
+lemma cp_dot_boss_at_pre: "((X).boss@pre) \<tau> = ((\<lambda>_. X \<tau>).boss@pre) \<tau>" by(simp add: eval_extract_def)
+
+lemma cp_dot_boss_pre: "((X).salary@pre) \<tau> = ((\<lambda>_. X \<tau>).salary@pre) \<tau>" by(simp add: eval_extract_def)
 
 lemmas cp_dot_bossI [simp, intro!]= 
        cp_dot_boss[THEN allI[THEN allI], of "\<lambda> X _. X" "\<lambda> _ \<tau>. \<tau>", THEN cpI1]
@@ -535,28 +548,23 @@ lemmas cp_dot_bossI_at_pre [simp, intro!]=
        cp_dot_boss_at_pre[THEN allI[THEN allI],  
                           of "\<lambda> X _. X" "\<lambda> _ \<tau>. \<tau>", THEN cpI1]
 
+
+
 lemma dot_boss_nullstrict [simp]: "(null).boss = invalid"
-by(rule ext, simp add: null_fun_def null_option_def bot_option_def null_def invalid_def)
+by(rule ext, simp add: null_fun_def null_option_def bot_option_def null_def invalid_def eval_extract_def)
 
 lemma dot_boss_at_pre_nullstrict [simp] : "(null).boss@pre = invalid"
-by(rule ext, simp add: null_fun_def null_option_def bot_option_def null_def invalid_def)
+by(rule ext, simp add: null_fun_def null_option_def bot_option_def null_def invalid_def eval_extract_def)
 
 lemma dot_boss_strict [simp] : "(invalid).boss = invalid" 
-by(rule ext, simp add: null_fun_def null_option_def bot_option_def null_def invalid_def)
+by(rule ext, simp add: null_fun_def null_option_def bot_option_def null_def invalid_def eval_extract_def)
 
 lemma dot_boss_at_pre_strict [simp] : "(invalid).boss@pre = invalid"
-by(rule ext, simp add: null_fun_def null_option_def bot_option_def null_def invalid_def)
+by(rule ext, simp add: null_fun_def null_option_def bot_option_def null_def invalid_def eval_extract_def)
+
+
 
 subsection{* A little infra-structure on example states.*}
-
-definition ocl_1000 ("\<one>\<zero>\<zero>\<zero>") where "ocl_1000 = (\<lambda> _ . \<lfloor>\<lfloor>1000\<rfloor>\<rfloor>)"
-definition ocl_1200 ("\<one>\<two>\<zero>\<zero>") where "ocl_1200 = (\<lambda> _ . \<lfloor>\<lfloor>1200\<rfloor>\<rfloor>)"
-definition ocl_1300 ("\<one>\<three>\<zero>\<zero>") where "ocl_1300 = (\<lambda> _ . \<lfloor>\<lfloor>1300\<rfloor>\<rfloor>)"
-definition ocl_1800 ("\<one>\<eight>\<zero>\<zero>") where "ocl_1800 = (\<lambda> _ . \<lfloor>\<lfloor>1800\<rfloor>\<rfloor>)"
-definition ocl_2600 ("\<two>\<six>\<zero>\<zero>") where "ocl_2600 = (\<lambda> _ . \<lfloor>\<lfloor>2600\<rfloor>\<rfloor>)"
-definition ocl_2900 ("\<two>\<nine>\<zero>\<zero>") where "ocl_2900 = (\<lambda> _ . \<lfloor>\<lfloor>2900\<rfloor>\<rfloor>)"
-definition ocl_3200 ("\<three>\<two>\<zero>\<zero>") where "ocl_3200 = (\<lambda> _ . \<lfloor>\<lfloor>3200\<rfloor>\<rfloor>)"
-definition ocl_3500 ("\<three>\<five>\<zero>\<zero>") where "ocl_3500 = (\<lambda> _ . \<lfloor>\<lfloor>3500\<rfloor>\<rfloor>)"
 
 definition "oid\<^isub>1 \<equiv> 0"
 definition "oid\<^isub>2 \<equiv> 1"
@@ -566,21 +574,21 @@ definition "oid\<^isub>5 \<equiv> 4"
 definition "oid\<^isub>6 \<equiv> 5"
 definition "oid\<^isub>7 \<equiv> 6"
 
-definition "person1 \<equiv> mk\<^isub>p\<^isub>e\<^isub>r\<^isub>s\<^isub>o\<^isub>n oid\<^isub>1 \<lfloor>1300\<rfloor> \<lfloor>oid\<^isub>2\<rfloor>"
-definition "person2 \<equiv> mk\<^isub>p\<^isub>e\<^isub>r\<^isub>s\<^isub>o\<^isub>n oid\<^isub>2 \<lfloor>1800\<rfloor> \<lfloor>oid\<^isub>2\<rfloor>"
+definition "person1 \<equiv> mk\<^isub>p\<^isub>e\<^isub>r\<^isub>s\<^isub>o\<^isub>n oid\<^isub>1 \<lfloor>2\<rfloor> \<lfloor>oid\<^isub>2\<rfloor>"
+definition "person2 \<equiv> mk\<^isub>p\<^isub>e\<^isub>r\<^isub>s\<^isub>o\<^isub>n oid\<^isub>2 \<lfloor>5\<rfloor> \<lfloor>oid\<^isub>2\<rfloor>"
 definition "person3 \<equiv> mk\<^isub>p\<^isub>e\<^isub>r\<^isub>s\<^isub>o\<^isub>n oid\<^isub>3 None None"
-definition "person4 \<equiv> mk\<^isub>p\<^isub>e\<^isub>r\<^isub>s\<^isub>o\<^isub>n oid\<^isub>4 \<lfloor>2900\<rfloor> None"
-definition "person5 \<equiv> mk\<^isub>p\<^isub>e\<^isub>r\<^isub>s\<^isub>o\<^isub>n oid\<^isub>5 \<lfloor>3500\<rfloor> None"
-definition "person6 \<equiv> mk\<^isub>p\<^isub>e\<^isub>r\<^isub>s\<^isub>o\<^isub>n oid\<^isub>6 \<lfloor>2500\<rfloor> \<lfloor>oid\<^isub>7\<rfloor>"
-definition "person7 \<equiv> mk\<^isub>o\<^isub>c\<^isub>l\<^isub>a\<^isub>n\<^isub>y oid\<^isub>7 \<lfloor>(\<lfloor>3200\<rfloor>, \<lfloor>oid\<^isub>7\<rfloor>)\<rfloor>"
+definition "person4 \<equiv> mk\<^isub>p\<^isub>e\<^isub>r\<^isub>s\<^isub>o\<^isub>n oid\<^isub>4 \<lfloor>8\<rfloor> None"
+definition "person5 \<equiv> mk\<^isub>p\<^isub>e\<^isub>r\<^isub>s\<^isub>o\<^isub>n oid\<^isub>5 \<lfloor>7\<rfloor> None"
+definition "person6 \<equiv> mk\<^isub>p\<^isub>e\<^isub>r\<^isub>s\<^isub>o\<^isub>n oid\<^isub>6 \<lfloor>11\<rfloor> \<lfloor>oid\<^isub>7\<rfloor>"
+definition "person7 \<equiv> mk\<^isub>o\<^isub>c\<^isub>l\<^isub>a\<^isub>n\<^isub>y oid\<^isub>7 \<lfloor>(\<lfloor>10\<rfloor>, \<lfloor>oid\<^isub>7\<rfloor>)\<rfloor>"
 
 definition 
-      "\<sigma>\<^isub>1  \<equiv> \<lparr> heap = empty(oid\<^isub>1 \<mapsto> in\<^isub>p\<^isub>e\<^isub>r\<^isub>s\<^isub>o\<^isub>n(mk\<^isub>p\<^isub>e\<^isub>r\<^isub>s\<^isub>o\<^isub>n oid\<^isub>1 \<lfloor>1000\<rfloor> \<lfloor>oid\<^isub>2\<rfloor>))
-                           (oid\<^isub>2 \<mapsto> in\<^isub>p\<^isub>e\<^isub>r\<^isub>s\<^isub>o\<^isub>n(mk\<^isub>p\<^isub>e\<^isub>r\<^isub>s\<^isub>o\<^isub>n oid\<^isub>2 \<lfloor>1200\<rfloor>  None))
+      "\<sigma>\<^isub>1  \<equiv> \<lparr> heap = empty(oid\<^isub>1 \<mapsto> in\<^isub>p\<^isub>e\<^isub>r\<^isub>s\<^isub>o\<^isub>n(mk\<^isub>p\<^isub>e\<^isub>r\<^isub>s\<^isub>o\<^isub>n oid\<^isub>1 \<lfloor>1\<rfloor> \<lfloor>oid\<^isub>2\<rfloor>))
+                           (oid\<^isub>2 \<mapsto> in\<^isub>p\<^isub>e\<^isub>r\<^isub>s\<^isub>o\<^isub>n(mk\<^isub>p\<^isub>e\<^isub>r\<^isub>s\<^isub>o\<^isub>n oid\<^isub>2 \<lfloor>3\<rfloor>  None))
                           (*oid\<^isub>3*)
-                           (oid\<^isub>4 \<mapsto> in\<^isub>p\<^isub>e\<^isub>r\<^isub>s\<^isub>o\<^isub>n(mk\<^isub>p\<^isub>e\<^isub>r\<^isub>s\<^isub>o\<^isub>n oid\<^isub>4 \<lfloor>2600\<rfloor> \<lfloor>oid\<^isub>5\<rfloor>))
+                           (oid\<^isub>4 \<mapsto> in\<^isub>p\<^isub>e\<^isub>r\<^isub>s\<^isub>o\<^isub>n(mk\<^isub>p\<^isub>e\<^isub>r\<^isub>s\<^isub>o\<^isub>n oid\<^isub>4 \<lfloor>6\<rfloor> \<lfloor>oid\<^isub>5\<rfloor>))
                            (oid\<^isub>5 \<mapsto> in\<^isub>p\<^isub>e\<^isub>r\<^isub>s\<^isub>o\<^isub>n person5)
-                           (oid\<^isub>6 \<mapsto> in\<^isub>p\<^isub>e\<^isub>r\<^isub>s\<^isub>o\<^isub>n(mk\<^isub>p\<^isub>e\<^isub>r\<^isub>s\<^isub>o\<^isub>n oid\<^isub>6 \<lfloor>2300\<rfloor> \<lfloor>oid\<^isub>4\<rfloor>)),
+                           (oid\<^isub>6 \<mapsto> in\<^isub>p\<^isub>e\<^isub>r\<^isub>s\<^isub>o\<^isub>n(mk\<^isub>p\<^isub>e\<^isub>r\<^isub>s\<^isub>o\<^isub>n oid\<^isub>6 \<lfloor>9\<rfloor> \<lfloor>oid\<^isub>4\<rfloor>)),
                assocs = empty\<rparr>"
 
 definition 
@@ -622,44 +630,37 @@ lemmas [code_unfold, simp] =
  oclastype\<^isub>p\<^isub>e\<^isub>r\<^isub>s\<^isub>o\<^isub>n_OclAny
  oclastype\<^isub>p\<^isub>e\<^isub>r\<^isub>s\<^isub>o\<^isub>n_Person
 
-value "\<not>((\<sigma>\<^isub>1,\<sigma>\<^isub>1') \<Turnstile>     ((X\<^isub>P\<^isub>e\<^isub>r\<^isub>s\<^isub>o\<^isub>n1 .salary)    \<doteq> \<one>\<zero>\<zero>\<zero> ))"
-value "  (\<sigma>\<^isub>1,\<sigma>\<^isub>1') \<Turnstile>     ((X\<^isub>P\<^isub>e\<^isub>r\<^isub>s\<^isub>o\<^isub>n1 .salary)    \<doteq> \<one>\<three>\<zero>\<zero> )"
-value "  (\<sigma>\<^isub>1,\<sigma>\<^isub>1') \<Turnstile>     ((X\<^isub>P\<^isub>e\<^isub>r\<^isub>s\<^isub>o\<^isub>n1 .salary@pre)     \<doteq> \<one>\<zero>\<zero>\<zero> )" 
-value "\<not>((\<sigma>\<^isub>1,\<sigma>\<^isub>1') \<Turnstile>     ((X\<^isub>P\<^isub>e\<^isub>r\<^isub>s\<^isub>o\<^isub>n1 .salary@pre)     \<doteq> \<one>\<three>\<zero>\<zero> ))"
+value "\<not>((\<sigma>\<^isub>1,\<sigma>\<^isub>1') \<Turnstile>     ((X\<^isub>P\<^isub>e\<^isub>r\<^isub>s\<^isub>o\<^isub>n1 .salary)    \<doteq> \<one> ))"
+value "  (\<sigma>\<^isub>1,\<sigma>\<^isub>1') \<Turnstile>     ((X\<^isub>P\<^isub>e\<^isub>r\<^isub>s\<^isub>o\<^isub>n1 .salary)    \<doteq> \<two> )"
+value "  (\<sigma>\<^isub>1,\<sigma>\<^isub>1') \<Turnstile>     ((X\<^isub>P\<^isub>e\<^isub>r\<^isub>s\<^isub>o\<^isub>n1 .salary@pre)     \<doteq> \<one>)" 
+value "\<not>((\<sigma>\<^isub>1,\<sigma>\<^isub>1') \<Turnstile>     ((X\<^isub>P\<^isub>e\<^isub>r\<^isub>s\<^isub>o\<^isub>n1 .salary@pre)     \<doteq> \<two> ))"
 value "\<not>((\<sigma>\<^isub>1,\<sigma>\<^isub>1') \<Turnstile>     ((X\<^isub>P\<^isub>e\<^isub>r\<^isub>s\<^isub>o\<^isub>n1 .boss )  \<doteq> X\<^isub>P\<^isub>e\<^isub>r\<^isub>s\<^isub>o\<^isub>n1 ))"
-value "  (\<sigma>\<^isub>1,\<sigma>\<^isub>1') \<Turnstile>     ((X\<^isub>P\<^isub>e\<^isub>r\<^isub>s\<^isub>o\<^isub>n1 .boss .salary)   \<doteq> \<one>\<eight>\<zero>\<zero> )"
+value "  (\<sigma>\<^isub>1,\<sigma>\<^isub>1') \<Turnstile>     ((X\<^isub>P\<^isub>e\<^isub>r\<^isub>s\<^isub>o\<^isub>n1 .boss .salary)   \<doteq> \<five> )"
 value "\<not>((\<sigma>\<^isub>1,\<sigma>\<^isub>1') \<Turnstile>     ((X\<^isub>P\<^isub>e\<^isub>r\<^isub>s\<^isub>o\<^isub>n1 .boss .boss)  \<doteq> X\<^isub>P\<^isub>e\<^isub>r\<^isub>s\<^isub>o\<^isub>n1 ))" 
-value "  (\<sigma>\<^isub>1,\<sigma>\<^isub>1') \<Turnstile>     ((X\<^isub>P\<^isub>e\<^isub>r\<^isub>s\<^isub>o\<^isub>n1 .boss .boss)  \<doteq> X\<^isub>P\<^isub>e\<^isub>r\<^isub>s\<^isub>o\<^isub>n2 )" 
-value "  (\<sigma>\<^isub>1,\<sigma>\<^isub>1') \<Turnstile>     ((X\<^isub>P\<^isub>e\<^isub>r\<^isub>s\<^isub>o\<^isub>n1 .boss@pre .salary)  \<doteq> \<one>\<eight>\<zero>\<zero> )"
-value "  (\<sigma>\<^isub>1,\<sigma>\<^isub>1') \<Turnstile>     ((X\<^isub>P\<^isub>e\<^isub>r\<^isub>s\<^isub>o\<^isub>n1 .boss@pre .salary@pre)  \<doteq> \<one>\<two>\<zero>\<zero> )"
-value "\<not>((\<sigma>\<^isub>1,\<sigma>\<^isub>1') \<Turnstile>     ((X\<^isub>P\<^isub>e\<^isub>r\<^isub>s\<^isub>o\<^isub>n1 .boss@pre .salary@pre)  \<doteq> \<one>\<eight>\<zero>\<zero> ))"
-value "  (\<sigma>\<^isub>1,\<sigma>\<^isub>1') \<Turnstile>     ((X\<^isub>P\<^isub>e\<^isub>r\<^isub>s\<^isub>o\<^isub>n1 .boss@pre)  \<doteq> X\<^isub>P\<^isub>e\<^isub>r\<^isub>s\<^isub>o\<^isub>n2 )"
+value "  (\<sigma>\<^isub>1,\<sigma>\<^isub>1') \<Turnstile>     ((X\<^isub>P\<^isub>e\<^isub>r\<^isub>s\<^isub>o\<^isub>n1 .boss@pre .salary)  \<doteq> \<five> )"
+value "  (\<sigma>\<^isub>1,\<sigma>\<^isub>1') \<Turnstile>     ((X\<^isub>P\<^isub>e\<^isub>r\<^isub>s\<^isub>o\<^isub>n1 .boss@pre .salary@pre)  \<doteq> \<three> )"
+value "\<not>((\<sigma>\<^isub>1,\<sigma>\<^isub>1') \<Turnstile>     ((X\<^isub>P\<^isub>e\<^isub>r\<^isub>s\<^isub>o\<^isub>n1 .boss@pre .salary@pre)  \<doteq> \<five> ))"
 value "  (\<sigma>\<^isub>1,\<sigma>\<^isub>1') \<Turnstile>     ((X\<^isub>P\<^isub>e\<^isub>r\<^isub>s\<^isub>o\<^isub>n1 .boss@pre .boss)  \<doteq> X\<^isub>P\<^isub>e\<^isub>r\<^isub>s\<^isub>o\<^isub>n2 )"
 value "  (\<sigma>\<^isub>1,\<sigma>\<^isub>1') \<Turnstile>     ((X\<^isub>P\<^isub>e\<^isub>r\<^isub>s\<^isub>o\<^isub>n1 .boss@pre .boss@pre)  \<doteq> null )"
 value "  (\<sigma>\<^isub>1,\<sigma>\<^isub>1') \<Turnstile> not(\<upsilon>(X\<^isub>P\<^isub>e\<^isub>r\<^isub>s\<^isub>o\<^isub>n1 .boss@pre .boss@pre .boss@pre))"
 
 
-value "  (\<sigma>\<^isub>1,\<sigma>\<^isub>1') \<Turnstile>     ((X\<^isub>P\<^isub>e\<^isub>r\<^isub>s\<^isub>o\<^isub>n2 .salary)       \<doteq> \<one>\<eight>\<zero>\<zero> )" 
-value "  (\<sigma>\<^isub>1,\<sigma>\<^isub>1') \<Turnstile>     ((X\<^isub>P\<^isub>e\<^isub>r\<^isub>s\<^isub>o\<^isub>n2 .salary@pre)   \<doteq> \<one>\<two>\<zero>\<zero> )" 
+value "  (\<sigma>\<^isub>1,\<sigma>\<^isub>1') \<Turnstile>     ((X\<^isub>P\<^isub>e\<^isub>r\<^isub>s\<^isub>o\<^isub>n2 .salary)       \<doteq> \<five>)" 
+value "  (\<sigma>\<^isub>1,\<sigma>\<^isub>1') \<Turnstile>     ((X\<^isub>P\<^isub>e\<^isub>r\<^isub>s\<^isub>o\<^isub>n2 .salary@pre)   \<doteq> \<three>)" 
 value "  (\<sigma>\<^isub>1,\<sigma>\<^isub>1') \<Turnstile>     ((X\<^isub>P\<^isub>e\<^isub>r\<^isub>s\<^isub>o\<^isub>n2 .boss)      \<doteq> X\<^isub>P\<^isub>e\<^isub>r\<^isub>s\<^isub>o\<^isub>n2)"
 value "  (\<sigma>\<^isub>1,\<sigma>\<^isub>1') \<Turnstile>     ((X\<^isub>P\<^isub>e\<^isub>r\<^isub>s\<^isub>o\<^isub>n2 .boss@pre)  \<doteq> null )"
 value "\<not>((\<sigma>\<^isub>1,\<sigma>\<^isub>1') \<Turnstile>     ((X\<^isub>P\<^isub>e\<^isub>r\<^isub>s\<^isub>o\<^isub>n2 .boss@pre)  \<doteq> X\<^isub>P\<^isub>e\<^isub>r\<^isub>s\<^isub>o\<^isub>n2))" 
 value "\<not>((\<sigma>\<^isub>1,\<sigma>\<^isub>1') \<Turnstile>     ((X\<^isub>P\<^isub>e\<^isub>r\<^isub>s\<^isub>o\<^isub>n2 .boss@pre)  \<doteq> (X\<^isub>P\<^isub>e\<^isub>r\<^isub>s\<^isub>o\<^isub>n2 .boss)))" 
-value "  (\<sigma>\<^isub>1,\<sigma>\<^isub>1') \<Turnstile> not(\<upsilon>(X\<^isub>P\<^isub>e\<^isub>r\<^isub>s\<^isub>o\<^isub>n2 .boss@pre .boss))"
-value "  (\<sigma>\<^isub>1,\<sigma>\<^isub>1') \<Turnstile> not(\<upsilon>(X\<^isub>P\<^isub>e\<^isub>r\<^isub>s\<^isub>o\<^isub>n2 .boss@pre .salary@pre))"
 
 
 value "  (\<sigma>\<^isub>1,\<sigma>\<^isub>1') \<Turnstile>     ((X\<^isub>P\<^isub>e\<^isub>r\<^isub>s\<^isub>o\<^isub>n3 .salary)       \<doteq> null)"
 value "  (\<sigma>\<^isub>1,\<sigma>\<^isub>1') \<Turnstile> not(\<upsilon>(X\<^isub>P\<^isub>e\<^isub>r\<^isub>s\<^isub>o\<^isub>n3 .salary@pre))"
 value "\<not>((\<sigma>\<^isub>1,\<sigma>\<^isub>1') \<Turnstile>     ((X\<^isub>P\<^isub>e\<^isub>r\<^isub>s\<^isub>o\<^isub>n3 .salary@pre)   \<doteq> null))"
-value "  (\<sigma>\<^isub>1,\<sigma>\<^isub>1') \<Turnstile>      (X\<^isub>P\<^isub>e\<^isub>r\<^isub>s\<^isub>o\<^isub>n3 .boss       \<doteq> null)"
-value "  (\<sigma>\<^isub>1,\<sigma>\<^isub>1') \<Turnstile> not(\<upsilon>(X\<^isub>P\<^isub>e\<^isub>r\<^isub>s\<^isub>o\<^isub>n3 .boss .salary))"
-value "  (\<sigma>\<^isub>1,\<sigma>\<^isub>1') \<Turnstile> not(\<upsilon>(X\<^isub>P\<^isub>e\<^isub>r\<^isub>s\<^isub>o\<^isub>n3 .boss@pre))"
 
 
 value "  (\<sigma>\<^isub>1,\<sigma>\<^isub>1') \<Turnstile>     ((X\<^isub>P\<^isub>e\<^isub>r\<^isub>s\<^isub>o\<^isub>n4 .boss@pre)   \<doteq> X\<^isub>P\<^isub>e\<^isub>r\<^isub>s\<^isub>o\<^isub>n5 )"
 value "  (\<sigma>\<^isub>1,\<sigma>\<^isub>1') \<Turnstile> not(\<upsilon>(X\<^isub>P\<^isub>e\<^isub>r\<^isub>s\<^isub>o\<^isub>n4 .boss@pre .salary))" 
-value "  (\<sigma>\<^isub>1,\<sigma>\<^isub>1') \<Turnstile>     ((X\<^isub>P\<^isub>e\<^isub>r\<^isub>s\<^isub>o\<^isub>n4 .boss@pre .salary@pre)   \<doteq> \<three>\<five>\<zero>\<zero> )"
+value "  (\<sigma>\<^isub>1,\<sigma>\<^isub>1') \<Turnstile>     ((X\<^isub>P\<^isub>e\<^isub>r\<^isub>s\<^isub>o\<^isub>n4 .boss@pre .salary@pre)   \<doteq> \<seven> )"
 lemma "  (\<sigma>\<^isub>1,\<sigma>\<^isub>1') \<Turnstile>   not(X\<^isub>P\<^isub>e\<^isub>r\<^isub>s\<^isub>o\<^isub>n4 .oclIsNew() )"
 by(simp add: not_def OclValid_def oclisnew_def 
              \<sigma>\<^isub>1_def \<sigma>\<^isub>1'_def
@@ -668,22 +669,22 @@ by(simp add: not_def OclValid_def oclisnew_def
              oid_of_option_def oid_of_person_def)
 
 
-value "\<not>((\<sigma>\<^isub>1,\<sigma>\<^isub>1') \<Turnstile>     ((X\<^isub>P\<^isub>e\<^isub>r\<^isub>s\<^isub>o\<^isub>n5 .salary)   \<doteq> \<three>\<five>\<zero>\<zero> ))"
-value "  (\<sigma>\<^isub>1,\<sigma>\<^isub>1') \<Turnstile>     ((X\<^isub>P\<^isub>e\<^isub>r\<^isub>s\<^isub>o\<^isub>n5 .salary@pre)   \<doteq> \<three>\<five>\<zero>\<zero> )"
+value "\<not>((\<sigma>\<^isub>1,\<sigma>\<^isub>1') \<Turnstile>     ((X\<^isub>P\<^isub>e\<^isub>r\<^isub>s\<^isub>o\<^isub>n5 .salary)   \<doteq> \<seven> ))"
+value "  (\<sigma>\<^isub>1,\<sigma>\<^isub>1') \<Turnstile>     ((X\<^isub>P\<^isub>e\<^isub>r\<^isub>s\<^isub>o\<^isub>n5 .salary@pre)   \<doteq> \<seven> )"
 
 
-value "  (\<sigma>\<^isub>1,\<sigma>\<^isub>1') \<Turnstile>     ((X\<^isub>P\<^isub>e\<^isub>r\<^isub>s\<^isub>o\<^isub>n6 .boss .salary)   \<doteq> \<three>\<two>\<zero>\<zero> )"
+value "  (\<sigma>\<^isub>1,\<sigma>\<^isub>1') \<Turnstile>     ((X\<^isub>P\<^isub>e\<^isub>r\<^isub>s\<^isub>o\<^isub>n6 .boss .salary)   \<doteq> \<one>\<zero> )"
 value "  (\<sigma>\<^isub>1,\<sigma>\<^isub>1') \<Turnstile> not(\<upsilon>(X\<^isub>P\<^isub>e\<^isub>r\<^isub>s\<^isub>o\<^isub>n6 .boss .salary@pre))" 
 value "  (\<sigma>\<^isub>1,\<sigma>\<^isub>1') \<Turnstile>     ((X\<^isub>P\<^isub>e\<^isub>r\<^isub>s\<^isub>o\<^isub>n6 .boss@pre)   \<doteq> X\<^isub>P\<^isub>e\<^isub>r\<^isub>s\<^isub>o\<^isub>n4 )"
-value "  (\<sigma>\<^isub>1,\<sigma>\<^isub>1') \<Turnstile>     ((X\<^isub>P\<^isub>e\<^isub>r\<^isub>s\<^isub>o\<^isub>n6 .boss@pre .salary)   \<doteq> \<two>\<nine>\<zero>\<zero> )"
-value "  (\<sigma>\<^isub>1,\<sigma>\<^isub>1') \<Turnstile>     ((X\<^isub>P\<^isub>e\<^isub>r\<^isub>s\<^isub>o\<^isub>n6 .boss@pre .salary@pre)   \<doteq> \<two>\<six>\<zero>\<zero> )"
+value "  (\<sigma>\<^isub>1,\<sigma>\<^isub>1') \<Turnstile>     ((X\<^isub>P\<^isub>e\<^isub>r\<^isub>s\<^isub>o\<^isub>n6 .boss@pre .salary)   \<doteq> \<eight> )"
+value "  (\<sigma>\<^isub>1,\<sigma>\<^isub>1') \<Turnstile>     ((X\<^isub>P\<^isub>e\<^isub>r\<^isub>s\<^isub>o\<^isub>n6 .boss@pre .salary@pre)   \<doteq> \<six> )"
 
 
 value "  (\<sigma>\<^isub>1,\<sigma>\<^isub>1') \<Turnstile>     ((X\<^isub>P\<^isub>e\<^isub>r\<^isub>s\<^isub>o\<^isub>n7 .oclAsType(Person)   \<doteq>  (X\<^isub>P\<^isub>e\<^isub>r\<^isub>s\<^isub>o\<^isub>n6 .boss)))"
 value "  (\<sigma>\<^isub>1,\<sigma>\<^isub>1') \<Turnstile>     ((X\<^isub>P\<^isub>e\<^isub>r\<^isub>s\<^isub>o\<^isub>n7 .oclAsType(Person) .boss)   \<doteq> (X\<^isub>P\<^isub>e\<^isub>r\<^isub>s\<^isub>o\<^isub>n7 .oclAsType(Person)) )"
-value "  (\<sigma>\<^isub>1,\<sigma>\<^isub>1') \<Turnstile>     ((X\<^isub>P\<^isub>e\<^isub>r\<^isub>s\<^isub>o\<^isub>n7 .oclAsType(Person) .boss .salary)   \<doteq> \<three>\<two>\<zero>\<zero> )"
 value "  (\<sigma>\<^isub>1,\<sigma>\<^isub>1') \<Turnstile> not(\<upsilon>(X\<^isub>P\<^isub>e\<^isub>r\<^isub>s\<^isub>o\<^isub>n7 .oclAsType(Person) .boss@pre))"
-value "  (\<sigma>\<^isub>1,\<sigma>\<^isub>1') \<Turnstile>     ((X\<^isub>P\<^isub>e\<^isub>r\<^isub>s\<^isub>o\<^isub>n7 .oclAsType(Person) .oclAsType(OclAny) .oclAsType(Person) )  \<doteq> (X\<^isub>P\<^isub>e\<^isub>r\<^isub>s\<^isub>o\<^isub>n7 .oclAsType(Person)) )"
+value "  (\<sigma>\<^isub>1,\<sigma>\<^isub>1') \<Turnstile>     ((X\<^isub>P\<^isub>e\<^isub>r\<^isub>s\<^isub>o\<^isub>n7 .oclAsType(Person) .oclAsType(OclAny) .oclAsType(Person) )  
+                          \<doteq> (X\<^isub>P\<^isub>e\<^isub>r\<^isub>s\<^isub>o\<^isub>n7 .oclAsType(Person)) )"
 lemma "  (\<sigma>\<^isub>1,\<sigma>\<^isub>1') \<Turnstile>      (X\<^isub>P\<^isub>e\<^isub>r\<^isub>s\<^isub>o\<^isub>n7 .oclIsNew() )"
 by(simp add: OclValid_def oclisnew_def 
              \<sigma>\<^isub>1_def \<sigma>\<^isub>1'_def
